Foundation/AutoProver/Litform.lean
@@ -5,13 +5,6 @@ import Mathlib.Tactic.TryThis
 import Mathlib.Util.AtomM
 import Foundation.Propositional.Hilbert.WellKnown
 
-inductive DbgResult (α : Type u) : α → Type u
-  | intro : (a b : α) → a = b → DbgResult α a
-
-instance {α} (a : α) : ToString (DbgResult α a) := ⟨fun r =>
-  match r with
-  | DbgResult.intro _ _ _ => "🎉 Proof Success! 🎉"⟩
-
 namespace Qq
 
 open Mathlib Qq Lean Elab Meta Tactic
@@ -31,12 +24,12 @@ lemma List.mem_singleton_of_eq (a b : α) (h : a = b) : a ∈ [b] := by simp [h]
 def memQList? {α : Q(Type u)} (a : Q($α)) : (l : List Q($α)) → MetaM <| Option Q($a ∈ $(toQList l))
   |     [] => return none
   | b :: l => do
-      if (← isDefEq (← whnf a) (← whnf b)) then
-        let e : Q($a = $b) := rflQ a
-        return some q(List.mem_of_eq $e)
-      else
-        let some h ← memQList? a l | return none
-        return some q(List.mem_of_mem $h)
+    if (← isDefEq (← whnf a) (← whnf b)) then
+      let e : Q($a = $b) := rflQ a
+      return some q(List.mem_of_eq $e)
+    else
+      let some h ← memQList? a l | return none
+      return some q(List.mem_of_mem $h)
 
 def memQList?' (a : Expr) (l : List Expr) : MetaM (Option Expr) := do
   let ⟨u, _, a⟩ ← inferTypeQ' a
@@ -71,9 +64,29 @@ lemma provable_of (h : [] ⟹ [φ]) : 𝓢 ⊢! φ :=
 lemma weakening (h : Γ₁ ⟹ Δ₁) (HΓ : Γ₁ ⊆ Γ₂ := by simp) (HΔ : Δ₁ ⊆ Δ₂ := by simp) : Γ₂ ⟹ Δ₂ :=
   FiniteContext.weakening! HΓ <| left_Disj!_intro Δ₁ (fun _ hψ ↦ right_Disj!_intro _ (HΔ hψ)) ⨀! h
 
-lemma rotate (hφ : Γ ⟹ Δ ++ [φ]) : Γ ⟹ φ :: Δ := weakening hφ
+lemma rotate_right (Γ Δ φ) (hφ : Γ ⟹ Δ ++ [φ]) : Γ ⟹ φ :: Δ := weakening hφ
 
-lemma and_right (Γ Δ φ ψ) (hφ : Γ ⟹ φ :: Δ) (hψ : Γ ⟹ ψ :: Δ) : Γ ⟹ φ ⋏ ψ :: Δ := by
+lemma rotate_left (Γ Δ φ) (hφ : (Γ ++ [φ]) ⟹ Δ) : (φ :: Γ) ⟹ Δ := weakening hφ
+
+lemma rotate_right_inv (Γ Δ φ) (hφ : Γ ⟹ φ :: Δ) : Γ ⟹ Δ ++ [φ] := weakening hφ
+
+lemma rotate_left_inv (Γ Δ φ) (hφ : (φ :: Γ) ⟹ Δ) : (Γ ++ [φ]) ⟹ Δ := weakening hφ
+
+variable (𝓢)
+
+lemma right_closed (Γ Δ φ) (h : φ ∈ Γ) : Γ ⟹ φ :: Δ := right_Disj!_intro _ (φ := φ) (by simp) ⨀! (by_axm! h)
+
+lemma left_closed (Γ Δ φ) (h : φ ∈ Δ) : (φ :: Γ) ⟹ Δ := right_Disj!_intro _ (φ := φ) h ⨀! by_axm!
+
+lemma verum_right (Γ Δ) : Γ ⟹ ⊤ :: Δ := right_Disj!_intro _ (φ := ⊤) (by simp) ⨀! (by simp)
+
+lemma falsum_left (Γ Δ) : (⊥ :: Γ) ⟹ Δ := efq! ⨀! by_axm₀!
+
+lemma falsum_right (Γ Δ) (h : Γ ⟹ Δ) : Γ ⟹ ⊥ :: Δ := weakening h
+
+lemma verum_left (Γ Δ) (h : Γ ⟹ Δ) : (⊤ :: Γ) ⟹ Δ := weakening h
+
+lemma and_right (Γ Δ φ ψ) (hφ : Γ ⟹ Δ ++ [φ]) (hψ : Γ ⟹ Δ ++ [ψ]) : Γ ⟹ φ ⋏ ψ :: Δ := by
   have : Γ ⊢[𝓢]! (φ :: Δ).disj ➝ (ψ :: Δ).disj ➝ (φ ⋏ ψ :: Δ).disj := by
     apply left_Disj!_intro
     rintro χ hχ
@@ -88,13 +101,99 @@ lemma and_right (Γ Δ φ ψ) (hφ : Γ ⟹ φ :: Δ) (hψ : Γ ⟹ ψ :: Δ) : 
     · apply deduct!
       apply dhyp!
       apply right_Disj!_intro _ (φ := χ) (by simp [hχ]) ⨀! by_axm₀!
-  exact this ⨀! hφ ⨀! hψ
+  exact this ⨀! rotate_right _ _ _ hφ ⨀! rotate_right _ _ _ hψ
 
-variable (𝓢)
+lemma or_left (Γ Δ φ ψ) (hφ : (Γ ++ [φ]) ⟹ Δ) (hψ : (Γ ++ [ψ]) ⟹ Δ) : (φ ⋎ ψ :: Γ) ⟹ Δ := by
+  apply deductInv!
+  apply left_A!_intro
+  · apply deduct! (rotate_left _ _ _ hφ)
+  · apply deduct! (rotate_left _ _ _ hψ)
 
-lemma right_closed (Γ φ Δ) (h : φ ∈ Γ) : Γ ⟹ φ :: Δ := right_Disj!_intro _ (φ := φ) (by simp) ⨀! (by_axm! h)
+lemma or_right (Γ Δ φ ψ) (h : Γ ⟹ Δ ++ [φ, ψ]) : Γ ⟹ φ ⋎ ψ :: Δ := by
+  have : Γ ⊢[𝓢]! (φ :: ψ :: Δ).disj ➝ (φ ⋎ ψ :: Δ).disj := by
+    apply left_Disj!_intro
+    intro χ hχ
+    rcases show χ = φ ∨ χ = ψ ∨ χ ∈ Δ by simpa using hχ with (rfl | rfl | hχ)
+    · apply right_Disj!_intro' (χ ⋎ ψ :: Δ) (φ := χ ⋎ ψ) (by simp) or₁!
+    · apply right_Disj!_intro' (φ ⋎ χ :: Δ) (φ := φ ⋎ χ) (by simp) or₂!
+    · apply right_Disj!_intro _ (by simp [hχ])
+  exact this ⨀! (weakening h)
 
-lemma left_closed (Γ φ Δ) (h : φ ∈ Δ) : (φ :: Γ) ⟹ Δ := right_Disj!_intro _ (φ := φ) h ⨀! by_axm!
+lemma and_left (Γ Δ φ ψ) (h : (Γ ++ [φ, ψ]) ⟹ Δ) : (φ ⋏ ψ :: Γ) ⟹ Δ := by
+  have h : (φ :: ψ :: Γ) ⟹ Δ := weakening h
+  have : (φ ⋏ ψ :: Γ) ⊢[𝓢]! ψ ➝ φ ➝ Δ.disj := wk! (by simp) (deduct! <| deduct! h)
+  exact this ⨀! (deductInv! and₂!) ⨀! (deductInv! and₁!)
+
+lemma neg_right (Γ Δ φ) (h : (Γ ++ [φ]) ⟹ Δ) : Γ ⟹ ∼φ :: Δ := by
+  have hφ : Γ ⊢[𝓢]! φ ➝ (∼φ :: Δ).disj := by
+    apply deduct!
+    suffices (φ :: Γ) ⊢[𝓢]! Δ.disj ➝ (∼φ :: Δ).disj from this ⨀ rotate_left Γ Δ φ h
+    apply left_Disj!_intro
+    intro ψ hψ
+    apply right_Disj!_intro _ (by simp [hψ])
+  have hnφ : Γ ⊢[𝓢]! ∼φ ➝ (∼φ :: Δ).disj := right_Disj!_intro _ (by simp)
+  exact left_A!_intro hφ hnφ ⨀ lem!
+
+lemma neg_left (Γ Δ φ) (h : Γ ⟹ Δ ++ [φ]) : (∼φ :: Γ) ⟹ Δ := by
+  suffices (∼φ :: Γ) ⊢[𝓢]! (φ :: Δ).disj ➝ Δ.disj from this ⨀ (wk! (by simp) (rotate_right _ _ _ h))
+  apply left_Disj!_intro
+  intro ψ hψ
+  rcases show ψ = φ ∨ ψ ∈ Δ by simpa using hψ with (rfl | hψ)
+  · apply deductInv!
+    exact CNC!
+  · apply right_Disj!_intro _ (by simp [hψ])
+
+lemma imply_right (Γ Δ φ ψ) (h : (Γ ++ [φ]) ⟹ Δ ++ [ψ]) : Γ ⟹ (φ ➝ ψ) :: Δ := by
+  have h : (φ :: Γ) ⟹ ψ :: Δ := weakening h
+  have hnφ : Γ ⊢[𝓢]! ∼φ ➝ ((φ ➝ ψ) :: Δ).disj := by
+    apply right_Disj!_intro' ((φ ➝ ψ) :: Δ) (φ := φ ➝ ψ) (by simp)
+    exact CNC!
+  have hφ : Γ ⊢[𝓢]! φ ➝ ((φ ➝ ψ) :: Δ).disj := by
+    apply deduct!
+    suffices (φ :: Γ) ⊢[𝓢]! (ψ :: Δ).disj ➝ ((φ ➝ ψ) :: Δ).disj from this ⨀ h
+    apply left_Disj!_intro
+    intro χ hχ
+    rcases show χ = ψ ∨ χ ∈ Δ by simpa using hχ with (rfl | hχ)
+    · apply right_Disj!_intro' _ (φ := φ ➝ χ) (by simp)
+      exact imply₁!
+    · apply right_Disj!_intro
+      simp [hχ]
+  exact left_A!_intro hφ hnφ ⨀ lem!
+
+lemma imply_left (Γ Δ φ ψ) (hφ : Γ ⟹ Δ ++ [φ]) (hψ : (Γ ++ [ψ]) ⟹ Δ) : ((φ ➝ ψ) :: Γ) ⟹ Δ := by
+  --apply deductInv!
+  suffices ((φ ➝ ψ) :: Γ) ⊢[𝓢]! (φ :: Δ).disj ➝ Δ.disj from this ⨀! wk! (by simp) (rotate_right Γ Δ φ hφ)
+  apply left_Disj!_intro
+  intro χ hχ
+  rcases show χ = φ ∨ χ ∈ Δ by simpa using hχ with (rfl | hχ)
+  · apply deduct!
+    have : Γ ⊢[𝓢]! ψ ➝ Δ.disj := deduct! (rotate_left Γ Δ ψ hψ)
+    apply (wk! (by simp) this) ⨀! (by_axm₁! ⨀! by_axm₀!)
+  · apply right_Disj!_intro _ (by simp [hχ])
+
+lemma iff_right (Γ Δ φ ψ) (hr : (Γ ++ [φ]) ⟹ Δ ++ [ψ]) (hl : (Γ ++ [ψ]) ⟹ Δ ++ [φ]) : Γ ⟹ (φ ⭤ ψ) :: Δ := by
+  apply and_right
+  · apply rotate_right_inv
+    apply imply_right
+    assumption
+  · apply rotate_right_inv
+    apply imply_right
+    assumption
+
+lemma iff_left (Γ Δ φ ψ) (hr : Γ ⟹ Δ ++ [φ, ψ]) (hl : (Γ ++ [φ, ψ]) ⟹ Δ) : ((φ ⭤ ψ) :: Γ) ⟹ Δ := by
+  apply and_left
+  suffices ((φ ➝ ψ) :: (ψ ➝ φ) :: Γ) ⟹ Δ from weakening this
+  apply imply_left
+  · apply imply_left
+    · simpa using hr
+    · suffices (φ :: Γ) ⟹ φ :: Δ from weakening this
+      apply deductInv!
+      apply right_Disj!_intro _ (by simp)
+  · apply imply_left
+    · suffices (ψ :: Γ) ⟹ ψ :: Δ from weakening this
+      apply deductInv!
+      apply right_Disj!_intro _ (by simp)
+    · exact weakening hl
 
 end TwoSided
 
@@ -126,9 +225,7 @@ instance : LogicalConnective (Litform α) where
 
 section ToString
 
-variable [ToString α]
-
-def toStr : Litform α → String
+def toStr [ToString α] : Litform α → String
   |       ⊤ => "⊤"
   |       ⊥ => "⊥"
   |  atom a => s!"atom {toString a}"
@@ -138,9 +235,20 @@ def toStr : Litform α → String
   |   φ ➝ ψ => "(" ++ toStr φ ++ " → "  ++ toStr ψ ++ ")"
   | iff φ ψ => "(" ++ toStr φ ++ " ↔ "  ++ toStr ψ ++ ")"
 
-instance : Repr (Litform α) := ⟨fun t _ => toStr t⟩
+instance [ToString α] : ToString (Litform α) := ⟨toStr⟩
 
-instance : ToString (Litform α) := ⟨toStr⟩
+
+def format [Repr α] : Litform α → Format
+  |       ⊤ => s!"⊤"
+  |       ⊥ => s!"⊥"
+  |  atom a => repr a
+  |      ∼φ => s!"(¬{format φ})"
+  |   φ ⋏ ψ => s!"({format φ} ∧ {format ψ})"
+  |   φ ⋎ ψ => s!"({format φ} ∨ {format ψ})"
+  |   φ ➝ ψ => s!"({format φ} → {format ψ})"
+  | iff φ ψ => s!"({format φ} ↔ {format ψ})"
+
+instance [Repr α] : Repr (Litform α) := ⟨fun t _ ↦ format t⟩
 
 end ToString
 
@@ -201,7 +309,6 @@ structure Context where
 /-- The monad for `cl_prover` contains. -/
 abbrev M := ReaderT Context AtomM
 
-#check Entailment.TwoSided.right_closed
 /-- Apply the function
   `n : ∀ {F} [LogicalConnective F] [DecidableEq F] {S} [Entailment F S] {𝓢} [Entailment.Cl 𝓢], _` to the
 implicit parameters in the context, and the given list of arguments. -/
@@ -237,29 +344,220 @@ def Sequent.toExpr (Γ : Sequent) : M Expr := do
   let c ← read
   return toQList <| Γ.map (Litform.toExpr c.LC)
 
-def code (Γ Δ : Sequent) : M Expr := do
-  match Δ with
-  |     [] => throwError m!"mssg: {Γ} ⟹ {Δ} found"
-  | φ :: Δ =>
-    logInfo m!"case: {φ} :: {Δ}"
-    match ← memQList?' (← Lit.toExpr φ) (← Γ.toExprList) with
-    | .none => throwError m! "FAILED: {φ} ∉ {Γ}"
-    | .some e => do
-      let eΔ ← Sequent.toExpr Δ
-      let eΓ ← Sequent.toExpr Γ
-      let eφ ← Lit.toExpr φ
-      logInfo m!"e : {e}"
-      let k ← iapp ``LO.Entailment.TwoSided.right_closed #[eΓ, eφ, eΔ, e]
-      logInfo m!"k : {k}"
-      iapp ``LO.Entailment.TwoSided.right_closed #[eΓ, eφ, eΔ, e]
+def tryRightClose (φ : Lit) (Γ Δ : Sequent) : M (Option Expr) := do
+  match ← memQList?' (← Lit.toExpr φ) (← Γ.toExprList) with
+  |   .none => return none
+  | .some e => do
+    let eΓ ← Sequent.toExpr Γ
+    let eΔ ← Sequent.toExpr Δ
+    let eφ ← Lit.toExpr φ
+    return some <| ← iapp ``LO.Entailment.TwoSided.right_closed #[eΓ, eΔ, eφ, e]
+
+def tryLeftClose (φ : Lit) (Γ Δ : Sequent) : M (Option Expr) := do
+  match ← memQList?' (← Lit.toExpr φ) (← Δ.toExprList) with
+  |   .none => return none
+  | .some e => do
+    let eΓ ← Sequent.toExpr Γ
+    let eΔ ← Sequent.toExpr Δ
+    let eφ ← Lit.toExpr φ
+    return some <| ← iapp ``LO.Entailment.TwoSided.left_closed #[eΓ, eΔ, eφ, e]
+
+def rotateRight (Γ Δ : Sequent) (φ : Lit) (e : Expr) : M Expr := do
+  let eΓ ← Sequent.toExpr Γ
+  let eΔ ← Sequent.toExpr Δ
+  let eφ ← Lit.toExpr φ
+  iapp ``LO.Entailment.TwoSided.rotate_right #[eΓ, eΔ, eφ, e]
+
+def rotateLeft (Γ Δ : Sequent) (φ : Lit) (e : Expr) : M Expr := do
+  let eΓ ← Sequent.toExpr Γ
+  let eΔ ← Sequent.toExpr Δ
+  let eφ ← Lit.toExpr φ
+  iapp ``LO.Entailment.TwoSided.rotate_left #[eΓ, eΔ, eφ, e]
+
+def verumRight (Γ Δ : Sequent) : M Expr := do
+  let eΓ ← Sequent.toExpr Γ
+  let eΔ ← Sequent.toExpr Δ
+  iapp ``LO.Entailment.TwoSided.verum_right #[eΓ, eΔ]
+
+def falsumRight (Γ Δ : Sequent) (e : Expr) : M Expr := do
+  let eΓ ← Sequent.toExpr Γ
+  let eΔ ← Sequent.toExpr Δ
+  iapp ``LO.Entailment.TwoSided.falsum_right #[eΓ, eΔ, e]
+
+def andRight (Γ Δ : Sequent) (φ ψ : Lit) (e₁ e₂ : Expr) : M Expr := do
+  let eΓ ← Sequent.toExpr Γ
+  let eΔ ← Sequent.toExpr Δ
+  let eφ ← Lit.toExpr φ
+  let eψ ← Lit.toExpr ψ
+  iapp ``LO.Entailment.TwoSided.and_right #[eΓ, eΔ, eφ, eψ, e₁, e₂]
+
+def orRight (Γ Δ : Sequent) (φ ψ : Lit) (e : Expr) : M Expr := do
+  let eΓ ← Sequent.toExpr Γ
+  let eΔ ← Sequent.toExpr Δ
+  let eφ ← Lit.toExpr φ
+  let eψ ← Lit.toExpr ψ
+  iapp ``LO.Entailment.TwoSided.or_right #[eΓ, eΔ, eφ, eψ, e]
+
+def negRight (Γ Δ : Sequent) (φ : Lit) (e : Expr) : M Expr := do
+  let eΓ ← Sequent.toExpr Γ
+  let eΔ ← Sequent.toExpr Δ
+  let eφ ← Lit.toExpr φ
+  iapp ``LO.Entailment.TwoSided.neg_right #[eΓ, eΔ, eφ, e]
+
+def implyRight (Γ Δ : Sequent) (φ ψ : Lit) (e : Expr) : M Expr := do
+  let eΓ ← Sequent.toExpr Γ
+  let eΔ ← Sequent.toExpr Δ
+  let eφ ← Lit.toExpr φ
+  let eψ ← Lit.toExpr ψ
+  iapp ``LO.Entailment.TwoSided.imply_right #[eΓ, eΔ, eφ, eψ, e]
+
+def iffRight (Γ Δ : Sequent) (φ ψ : Lit) (e₁ e₂ : Expr) : M Expr := do
+  let eΓ ← Sequent.toExpr Γ
+  let eΔ ← Sequent.toExpr Δ
+  let eφ ← Lit.toExpr φ
+  let eψ ← Lit.toExpr ψ
+  iapp ``LO.Entailment.TwoSided.iff_right #[eΓ, eΔ, eφ, eψ, e₁, e₂]
 
 
-elab "test2s" : tactic => withMainContext do
+def verumLeft (Γ Δ : Sequent) (e : Expr) : M Expr := do
+  let eΓ ← Sequent.toExpr Γ
+  let eΔ ← Sequent.toExpr Δ
+  iapp ``LO.Entailment.TwoSided.verum_left #[eΓ, eΔ, e]
+
+def falsumLeft (Γ Δ : Sequent) : M Expr := do
+  let eΓ ← Sequent.toExpr Γ
+  let eΔ ← Sequent.toExpr Δ
+  iapp ``LO.Entailment.TwoSided.falsum_left #[eΓ, eΔ]
+
+def andLeft (Γ Δ : Sequent) (φ ψ : Lit) (e : Expr) : M Expr := do
+  let eΓ ← Sequent.toExpr Γ
+  let eΔ ← Sequent.toExpr Δ
+  let eφ ← Lit.toExpr φ
+  let eψ ← Lit.toExpr ψ
+  iapp ``LO.Entailment.TwoSided.and_left #[eΓ, eΔ, eφ, eψ, e]
+
+def orLeft (Γ Δ : Sequent) (φ ψ : Lit) (e₁ e₂ : Expr) : M Expr := do
+  let eΓ ← Sequent.toExpr Γ
+  let eΔ ← Sequent.toExpr Δ
+  let eφ ← Lit.toExpr φ
+  let eψ ← Lit.toExpr ψ
+  iapp ``LO.Entailment.TwoSided.or_left #[eΓ, eΔ, eφ, eψ, e₁, e₂]
+
+def negLeft (Γ Δ : Sequent) (φ : Lit) (e : Expr) : M Expr := do
+  let eΓ ← Sequent.toExpr Γ
+  let eΔ ← Sequent.toExpr Δ
+  let eφ ← Lit.toExpr φ
+  iapp ``LO.Entailment.TwoSided.neg_left #[eΓ, eΔ, eφ, e]
+
+def implyLeft (Γ Δ : Sequent) (φ ψ : Lit) (e₁ e₂ : Expr) : M Expr := do
+  let eΓ ← Sequent.toExpr Γ
+  let eΔ ← Sequent.toExpr Δ
+  let eφ ← Lit.toExpr φ
+  let eψ ← Lit.toExpr ψ
+  iapp ``LO.Entailment.TwoSided.imply_left #[eΓ, eΔ, eφ, eψ, e₁, e₂]
+
+def iffLeft (Γ Δ : Sequent) (φ ψ : Lit) (e₁ e₂ : Expr) : M Expr := do
+  let eΓ ← Sequent.toExpr Γ
+  let eΔ ← Sequent.toExpr Δ
+  let eφ ← Lit.toExpr φ
+  let eψ ← Lit.toExpr ψ
+  iapp ``LO.Entailment.TwoSided.iff_left #[eΓ, eΔ, eφ, eψ, e₁, e₂]
+
+def search (k : ℕ) (b : Bool) (Γ Δ : Sequent) : M Expr := do
+  logInfo m!"step: {k}, case: {b}, {Γ} ⟹ {Δ}"
+  match k, b with
+  |     0,      _ => throwError m!"auto prove failed: {Γ} ⟹ {Δ}"
+  | k + 1,  false =>
+    match Δ with
+    |    .atom a :: Δ => do
+      let e ← tryRightClose (.atom a) Γ Δ
+      match e with
+      | some h =>
+        logInfo m!"case: GOAL CLOSED R: {a}"
+        return h
+      |   none => do
+        let e ← search k true Γ (Δ ++ [.atom a])
+        rotateRight Γ Δ (.atom a) e
+    |          ⊤ :: Δ => verumRight Γ Δ
+    |          ⊥ :: Δ => do
+      logInfo m!"case: ⊥_R"
+      let e ← search k true Γ Δ
+      falsumRight Γ Δ e
+    |      φ ⋏ ψ :: Δ => do
+      let e₁ ← search k true Γ (Δ ++ [φ])
+      let e₂ ← search k true Γ (Δ ++ [ψ])
+      andRight Γ Δ φ ψ e₁ e₂
+    |      φ ⋎ ψ :: Δ => do
+      let e ← search k true Γ (Δ ++ [φ, ψ])
+      orRight Γ Δ φ ψ e
+    |         ∼φ :: Δ => do
+      let e ← search k true (Γ ++ [φ]) Δ
+      negRight Γ Δ φ e
+    |    (φ ➝ ψ) :: Δ => do
+      logInfo m!"case: imply_R"
+      let e ← search k true (Γ ++ [φ]) (Δ ++ [ψ])
+      implyRight Γ Δ φ ψ e
+    | (.iff φ ψ) :: Δ => do
+      logInfo m!"case: iff_R"
+      let e₁ ← search k true (Γ ++ [φ]) (Δ ++ [ψ])
+      let e₂ ← search k true (Γ ++ [ψ]) (Δ ++ [φ])
+      iffRight Γ Δ φ ψ e₁ e₂
+    |              [] =>
+      search k true Γ []
+  | k + 1, true =>
+    match Γ with
+    |    .atom a :: Γ => do
+      let e ← tryLeftClose (.atom a) Γ Δ
+      match e with
+      | some h =>
+        logInfo m!"case: GOAL CLOSED L: {a}"
+        return h
+      |   none => do
+        let e ← search k false (Γ ++ [.atom a]) Δ
+        rotateLeft Γ Δ (.atom a) e
+    |          ⊤ :: Γ => do
+      let e ← search k false Γ Δ
+      verumLeft Γ Δ e
+    |          ⊥ :: Γ => do
+      falsumLeft Γ Δ
+    |      φ ⋏ ψ :: Γ => do
+      let e ← search k false (Γ ++ [φ, ψ]) Δ
+      andLeft Γ Δ φ ψ e
+    |      φ ⋎ ψ :: Γ => do
+      let e₁ ← search k false (Γ ++ [φ]) Δ
+      let e₂ ← search k false (Γ ++ [ψ]) Δ
+      orLeft Γ Δ φ ψ e₁ e₂
+    |         ∼φ :: Γ => do
+      let e ← search k false Γ (Δ ++ [φ])
+      negLeft Γ Δ φ e
+    |    (φ ➝ ψ) :: Γ => do
+      logInfo m!"case: imply_L"
+      let e₁ ← search k false Γ (Δ ++ [φ])
+      let e₂ ← search k false (Γ ++ [ψ]) Δ
+      implyLeft Γ Δ φ ψ e₁ e₂
+    | (.iff φ ψ) :: Γ => do
+      logInfo m!"case: iff_L"
+      let e₁ ← search k false Γ (Δ ++ [φ, ψ])
+      let e₂ ← search k false (Γ ++ [φ, ψ]) Δ
+      iffLeft Γ Δ φ ψ e₁ e₂
+    |              [] =>
+      search k false [] Δ
+
+elab "cl_prover_2s" n:(num)? : tactic => withMainContext do
+  let n : ℕ :=
+    match n with
+    | some n => n.getNat
+    | none   => 32
   let ⟨c, L, R⟩ ← getGoalTwoSided <| ← whnfR <| ← getMainTarget
   let Γ ← L.mapM (m := MetaM) (Litform.denote c.LC)
   let Δ ← R.mapM (m := MetaM) (Litform.denote c.LC)
-  logInfo m!"{Γ} ⟹ {Δ}"
-  closeMainGoal `cl_prover <| ← AtomM.run .reducible <| ReaderT.run (code Γ Δ) c
+  --logInfo m!"{Γ} ⟹ {Δ}"
+  closeMainGoal `cl_prover <| ← AtomM.run .reducible <| ReaderT.run (search n false Γ Δ) c
+
+macro "cl_prover" n:(num)? : tactic => do
+  match n with
+  | some n => `(tactic| apply LO.Entailment.TwoSided.provable_of <;> cl_prover_2s $n)
+  | none   => `(tactic| apply LO.Entailment.TwoSided.provable_of <;> cl_prover_2s)
 
 section
 
@@ -269,7 +567,19 @@ variable {F : Type*} [DecidableEq F] {S : Type*} [LogicalConnective F] [Entailme
 
 variable {𝓢 : S} [Entailment.Cl 𝓢] {φ ψ : F}
 
-example : Entailment.TwoSided 𝓢 [φ ⋏ ⊤, ψ] [ψ, φ] := by { test2s }
+example : Entailment.TwoSided 𝓢 [φ, ψ] [χ ⋏ ξ, χ, ψ] := by cl_prover_2s
+
+example : Entailment.TwoSided 𝓢 [φ ⭤ ψ] [φ ➝ (χ ⋎ ψ)] := by cl_prover_2s
+
+example : Entailment.TwoSided 𝓢 [⊥] [⊥] := by cl_prover_2s
+
+example : Entailment.TwoSided 𝓢 [φ ⭤ ψ, χ ⭤ ξ] [(ψ ➝ ξ) ⭤ (φ ➝ χ)] := by cl_prover_2s 32
+
+example : 𝓢 ⊢! (φ ⋏ ψ) ➝ ((φ ➝ ψ ➝ ⊥) ➝ ⊥) := by
+  cl_prover
+
+example : 𝓢 ⊢! ((φ ⭤ ψ) ⋏ (χ ⭤ ξ)) ➝ ((ψ ➝ ξ) ⭤ (φ ➝ χ)) := by
+  cl_prover
 
 end
 section
@@ -278,7 +588,7 @@ open LO.Propositional
 
 variable {φ ψ χ : Formula ℕ}
 
-example : Entailment.TwoSided Hilbert.Cl [φ ⋏ ⊤, ψ] [ψ, φ, .atom 9] := by { test2s }
+example : Entailment.TwoSided Hilbert.Cl [φ ⋏ ⊤, ψ] [ψ, φ, .atom 9] := by { cl_prover_2s }
 
 end
 
